SizeLemmas.v
@@ -8,8 +8,6 @@ Require Import Omega.
 (* see file ReducibilityMeasure for the full measure *)
 Fixpoint typeNodes T: nat :=
   match T with
-  | ite b T1 T2 => 1 + typeNodes T1 + typeNodes T2
-
   | T_unit => 0
   | T_bool => 0
   | T_nat => 0
@@ -29,7 +27,6 @@ Fixpoint typeNodes T: nat :=
   | T_exists A B => 1 + typeNodes A + typeNodes B
   | T_abs T => 1 + typeNodes T
   | T_rec _ T0 Ts => 1 + typeNodes T0 + typeNodes Ts
-  | T_interpret T => 1 + typeNodes T
 
   | _ => 0
   end.
@@ -77,66 +74,3 @@ Proof.
 Qed.
 
 Hint Rewrite typeNodes_swap: bsize.
-
-Fixpoint count_interpret (t: tree): nat :=
-  match t with
-  | ite b T1 T2 => count_interpret T1 + count_interpret T2
-
-  | T_refine A p => count_interpret A
-  | T_type_refine A B => count_interpret A + count_interpret B
-  | T_prod A B => count_interpret A + count_interpret B
-  | T_arrow A B => count_interpret A + count_interpret B
-  | T_sum A B => count_interpret A + count_interpret B
-  | T_let t B => count_interpret B
-  | T_intersection A B => count_interpret A + count_interpret B
-  | T_union A B => count_interpret A + count_interpret B
-  | T_forall A B => count_interpret A + count_interpret B
-  | T_exists A B => count_interpret A + count_interpret B
-  | T_abs T => count_interpret T
-  | T_rec n T0 Ts => count_interpret T0 + count_interpret Ts
-  | T_interpret t => 1 + count_interpret t
-  | _ => 0
-  end.
-
-(*
-Lemma count_interpret_term:
-  forall t, is_erased_term t -> count_interpret t = 0.
-Proof.
-  destruct t; steps.
-Qed.
-*)
-
-Lemma count_interpret_open:
-  forall T k rep,
-    is_erased_type T ->
-    is_erased_term rep ->
-    count_interpret (open k T rep) = count_interpret T.
-Proof.
-  induction T; repeat step || rewrite_any; try omega.
-Qed.
-
-Hint Rewrite count_interpret_open: bsize.
-
-Lemma count_interpret_open_var:
-  forall T k X, count_interpret (open k T (fvar X type_var)) = count_interpret T.
-Proof.
-  induction T; steps.
-Qed.
-
-Hint Rewrite count_interpret_open_var: bsize.
-
-Lemma count_interpret_topen_var:
-  forall T k X, count_interpret (topen k T (fvar X type_var)) = count_interpret T.
-Proof.
-  induction T; steps.
-Qed.
-
-Hint Rewrite count_interpret_topen_var: bsize.
-
-Lemma count_interpret_swap:
-  forall t i j, count_interpret (swap_type_holes t i j) = count_interpret t.
-Proof.
-  induction t; steps.
-Qed.
-
-Hint Rewrite count_interpret_swap: bsize.
